\section{$(a+b)^2$}
The square of the sum of two numbers is
\[(a+b)^2 = a^2 +2ab +b^2\]

\subsection{Derivation}
\begin{center}
\includegraphics[width=8cm]{Algebra/binomial_square_diag1}
\end{center}
The area of the square above is \((a+b)^2\) \\
It is also the sum of the 4 individual squares\\
\begin{align*}
(a+b)^2 &= aa + ab + ab + bb\\
(a+b)^2 &= a^2 +2ab + b^2
\end{align*}

\section{$(a+b)^3$}

\section{Binomial Theorem}

\section{Quadratic Equation}
The Quadratic Equation is most commonly stated as \\\\
Given the second order polynominal, \(ax^2 + bx + c = 0\)\\
the roots of equation are, \(x = \dfrac{-b \pm \sqrt{b^2 -4ac}}{2a}\) \\
but \(a \ne 0\)

\subsection{Derivation}

Let's rewrite \(ax^2+bx+c = 0 \) using the technique of Completing the Square \\
\begin{align*}
x^2 + \frac{b}{a} + \frac{c}{a} &= 0 \\
x^2 + \frac{b}{a} &= -\frac{c}{a} \\
x^2 + \frac{b}{a} + \left(\frac{1}{2}\frac{b}{a}\right)^2 &= -\frac{c}{a} + \left(\frac{1}{2}\frac{b}{a}\right)^2 \\
\left(x + \frac{b}{2a}\right)^2 &= -\frac{c}{a} + \frac{b^2}{4a^2} \\
\left(x + \frac{b}{2a}\right)^2 &= \frac{-4ac +b^2}{4a^2} \\
\end{align*}
Now just solve for x
\begin{align*}
x + \frac{b}{2a} &= \sqrt{\frac{b^2 -4ac}{4a^2}} \\
x  &= -\frac{b}{2a} \pm \sqrt{\frac{b^2 -4ac}{4a^2}}  \\
x &= \dfrac{-b \pm \sqrt{b^2 -4ac}}{2a}
\end{align*}
