\section{Integration by Parts}
Integration by parts is most commonly stated as
\[\int{udv} = uv - \int{vdu}\]
Where both the functions u and v are implied to be functions of another variable, u(x) and v(x)

\subsection{Derivation}
Integration by parts can be derived starting with the Product Rule
\begin{align*}
d\left[ u(x)v(x) \right] &= \frac{du}{dx}v(x) + u(x)\frac{dv}{dx} \\
\int{d\left[ u(x)v(x) \right]dx} &= \int{\left(\frac{du}{dx}v(x) + u(x)\frac{dv}{dx}\right)dx} \\
u(x)v(x) &= \int{\frac{du}{dx}v(x)dx} + \int{u(x)\frac{dv}{dx}dx} \\
u(x)v(x) - \int{\frac{du}{dx}v(x)dx} &=  \int{u(x)\frac{dv}{dx}dx} \\
\int{u(x)dv} &= u(x)v(x) - \int{v(x)du} \\
\end{align*}
Or more informally written as
\begin{align*}
\int{udv} &= uv - \int{vdu} 
\end{align*}
